> [!teorema] Probabilità dell'evento nullo
> $\mathbb{P}(\emptyset)=0$
> > [!dimostrazione]-
> > $\mathbb{P}(S)=1$, $S\cap \emptyset=\emptyset\implies \mathbb{P}(S\cup \emptyset)=\mathbb{P}(S)+\mathbb{P}(\emptyset)=1+\mathbb{P}(\emptyset)$

> [!teorema] Teorema delle probabilità totali
> $A,B$ eventi
> $\mathbb{P}(B)=\mathbb{P}(A\cap B)+\mathbb{P}(\bar{A}\cap B)$
> > [!dimostrazione]-
> $B=B\cap(A\cup \bar{A})=(B\cap A)\cup(B\cap \bar{A})$
> $\mathbb{P}((B\cap A)\cup(B\cap \bar{A})=\mathbb{P}(B\cap A)+\mathbb{P}(B\cap \bar{A})=\mathbb{P}(B)$

> [!teorema]
> $A,B$ eventi
> $\mathbb{P}(A\cup B)=\mathbb{P}(A)+\mathbb{P}(B)-\mathbb{P}(A\cap B)$

> [!teorema]
> Se $B\subset A\implies \mathbb{P}(B)\leq \mathbb{P}(A)$
> > [!dimostrazione]-
> > $\mathbb{P}(A)=\mathbb{P}(B)+\mathbb{P}(A\cap \bar{B})\geq \mathbb{P}(B)$
